{
 "cells": [
  {
   "cell_type": "markdown",
   "id": "6cd7162c",
   "metadata": {},
   "source": [
    "(ref:lec6:ex3_sol)=\n",
    "# Solutions of Exercise 6.3"
   ]
  },
  {
   "cell_type": "markdown",
   "id": "f8defabe",
   "metadata": {},
   "source": [
    "Consider the system in {numref}`fig:lec6:ex3_sol:block`.\n",
    "\n",
    "1. Find the state-space form of the system, where the states are $x_1$ and $x_2$ given in the figure.\n",
    "2. Compute a state-feedback controller for the state-space system defined in question 1, so that\n",
    "    - The closed-loop eigenvalues are placed in $-4$\n",
    "    - The static gain is exactly $1$\n",
    "\n",
    "\n",
    "```{figure} res/ex3-block.svg\n",
    "---\n",
    "width: 600px\n",
    "name: fig:lec6:ex3_sol:block\n",
    "---\n",
    "Block diagram of the system\n",
    "```"
   ]
  },
  {
   "cell_type": "markdown",
   "id": "1a6e6aa4",
   "metadata": {},
   "source": [
    "---"
   ]
  },
  {
   "cell_type": "markdown",
   "id": "9c9a9fa7",
   "metadata": {},
   "source": [
    "## Solution\n",
    "### Question 1\n",
    "\n",
    "Remembering that $s X(s)$ is equivalent to the derivative in the time domain, we can write\n",
    "\n",
    "$\n",
    "X_1(s) = \\frac{1}{s+1} U(s) \\quad \\rightarrow \\quad (s+1) X_1(s) = U(s) \\quad \\rightarrow \\quad \\dot{x}_1(t) + x_1(t) = u(t) \n",
    "$\n",
    "\n",
    "The first state evolves according to $\\dot{x}_1 = - x_1 + u$.\n",
    "\n",
    "When it comes to the second state,\n",
    "\n",
    "$\n",
    "X_2(s) = \\frac{1}{s+3} (U(s) + X_1(s))  \\quad \\rightarrow \\quad  (s+3) X_2(s) = U(s) + X_1(s) \\quad \\rightarrow \\quad \\dot{x}_2 = x_1 - 3 x_2 + u\n",
    "$\n",
    "\n",
    "Noting that $y = x_1 + x_2$, we can finally write the state-space system as\n",
    "\n",
    "$$\n",
    "\\begin{dcases}\n",
    "\\begin{bmatrix} \\dot{x}_1 \\\\ \\dot{x}_2 \\end{bmatrix} = \\begin{bmatrix} -1 & 0 \\\\ 1 & -3 \\end{bmatrix} \\begin{bmatrix} x_1 \\\\ x_2 \\end{bmatrix}  + \\begin{bmatrix} 1 \\\\ 1 \\end{bmatrix} u \\\\\n",
    "y = \\begin{bmatrix} 1 & 1 \\end{bmatrix} \\begin{bmatrix} x_1 \\\\ x_2 \\end{bmatrix}\n",
    "\\end{dcases}\n",
    "$$"
   ]
  },
  {
   "cell_type": "markdown",
   "id": "220b0a91",
   "metadata": {},
   "source": [
    "### Question 2\n",
    "\n",
    "To design a state-feedback controller $u = - L x + \\ell_0 r$, we first need to check the  controllability of the system\n",
    "\n",
    "$$\n",
    "    \\mathcal{S} = \\begin{bmatrix} B & AB \\end{bmatrix} = \\begin{bmatrix} 1 & -1 \\\\ 1 & -2 \\end{bmatrix}\n",
    "$$\n",
    "\n",
    "This matrix is full rank ($\\det(\\mathcal{S}) = -1 \\neq 0$), which means that the system is controllable. We can therefore design the state feedback controller, and we start by the gain $L$."
   ]
  },
  {
   "cell_type": "markdown",
   "id": "1300e600",
   "metadata": {},
   "source": [
    "Under the control law $u = - Lx + \\ell_0 r$, the closed-loop system is \n",
    "\n",
    "$\n",
    "\\dot{x} = A x + B (-Lx + \\ell_0 r) = (A - BL) x + B \\ell_0 r\n",
    "$\n",
    "\n",
    "The poles of the closed-loop are the eigenvalues of $A-BL$ which, of course, depend upon the controller's parameters, $L = \\begin{bmatrix} \\ell_1 & \\ell_2 \\end{bmatrix}$. To design the controller, we first write the characteristic polynomial of the closed-loop:\n",
    "\n",
    "$$\n",
    "\\begin{aligned}\n",
    "    \\varphi(\\lambda) &= \\det(\\lambda I - (A - BL)) = \\det\\left( \\begin{bmatrix} \\lambda & 0 \\\\ 0 & \\lambda \\end{bmatrix} - \\begin{bmatrix} -1 & 0 \\\\ 1 & -3 \\end{bmatrix} + \\begin{bmatrix} 1  \\\\ 1 \\end{bmatrix} \\begin{bmatrix} \\ell_1 & \\ell_2 \\end{bmatrix}\\right) \\\\\n",
    "    &= \\det \\begin{bmatrix} \\lambda + 1 + \\ell_1 & \\ell_2 \\\\ \\ell_1 - 1 & \\lambda + 3 + \\ell_2 \\end{bmatrix} \\\\\n",
    "    &= (\\lambda + 1 + \\ell_1) \\cdot (\\lambda + 3 + \\ell_2 ) - \\ell_2 (\\ell_1 - 1) \\\\\n",
    "    &= \\lambda^2 + (4 + \\ell_1 + \\ell_2) \\lambda + 3 + 3 \\ell_1 + 2 \\ell_2\n",
    "\\end{aligned}\n",
    "$$ (eq:lec6:ex3_sol:poly)"
   ]
  },
  {
   "cell_type": "markdown",
   "id": "381b072d",
   "metadata": {},
   "source": [
    "To find $\\ell_1$ and $\\ell_2$, we set the coefficients of this polynomial equal to the coefficients of the **desired characteristic polynomial**, i.e., the polynomial whose roots match the desired poles ($-4$ and $-4$):\n",
    "\n",
    "$$\n",
    "\\varphi^{\\star}(\\lambda) = (\\lambda+4)^2 = \\lambda^2 + 8 \\lambda +16\n",
    "$$ (eq:lec6:ex3_sol:desired_poly)\n",
    "\n",
    "By setting the coefficients of {eq}`eq:lec6:ex3_sol:poly` and {eq}`eq:lec6:ex3_sol:desired_poly` equal, we get\n",
    "\n",
    "$$\n",
    "\\begin{dcases}\n",
    "4 + \\ell_1 + \\ell_2 = 8 \\\\\n",
    "3 + 3 \\ell_1 + 2 \\ell_2 = 16\n",
    "\\end{dcases}\n",
    "$$"
   ]
  },
  {
   "cell_type": "markdown",
   "id": "4f92d2b7",
   "metadata": {},
   "source": [
    "From the first equation we get $\\ell_1 = 4 - \\ell_2$. Substituting this int othe second equation we obtain \n",
    "\n",
    "$\n",
    "3 + 3(4 - \\ell_2) + 2 \\ell_2 = 16 \\quad \\rightarrow \\quad -\\ell_2 = 16 - 15   \\quad \\rightarrow \\quad \\ell_2 = -1\n",
    "$\n",
    "\n",
    "We can now replace this $\\ell_2$ in the expression of $\\ell_1$, thus obtaining $\\ell_1 = 4 - (-1) = 5$.\n",
    "The state-feedback gain is therefore\n",
    "\n",
    "$$\n",
    "L = \\begin{bmatrix} 5 & -1 \\end{bmatrix}\n",
    "$$"
   ]
  },
  {
   "cell_type": "markdown",
   "id": "ea586334",
   "metadata": {},
   "source": [
    "The last parameter to find is $\\ell_0$. We design $\\ell_0$ so that the closed loop transfer function has a static gain equal to one.\n",
    "\n",
    "$$\n",
    "\\frac{Y(s)}{R(s)} = G_c(s) = C (sI - (A-BL))^{-1} B \\ell_0 $$"
   ]
  },
  {
   "cell_type": "markdown",
   "id": "25f82710",
   "metadata": {},
   "source": [
    "We now find $\\ell_0$ by enforcing $G_c(0) = 1$.\n",
    "\n",
    "$$\n",
    "-C (A - BL)^{-1} B \\ell_0 = 1 \\quad \\rightarrow \\quad \\ell_0 = -\\frac{1}{C (A-BL)^{-1} B}\n",
    "$$\n",
    "\n",
    "Let's compute $\\ell_0$ step-by-step.\n",
    "\n",
    "$\n",
    "A - BL = \\begin{bmatrix} -1 & 0 \\\\ 1 & -3 \\end{bmatrix} - \\begin{bmatrix} 1 \\\\ 1 \\end{bmatrix} \\begin{bmatrix} 5 & -1 \\end{bmatrix} = \\begin{bmatrix} -6 & 1 \\\\ -4 & -2 \\end{bmatrix}\n",
    "$\n",
    "\n",
    "$\n",
    "(A - BL)^{-1} = \\begin{bmatrix} -6 & 1 \\\\ -4 & -2 \\end{bmatrix}^{-1} = \\frac{1}{16} \\begin{bmatrix} -2 & -1 \\\\ 4 & -6 \\end{bmatrix}\n",
    "$\n",
    "\n",
    "$\n",
    "\\ell_0 = -\\frac{1}{\\frac{1}{16} \\begin{bmatrix} 1 & 1 \\end{bmatrix} \\begin{bmatrix} -2 & -1 \\\\ 4 & -6 \\end{bmatrix} \\begin{bmatrix} 1 & 1 \\end{bmatrix}} = -\\frac{16}{\\begin{bmatrix} 1 & 1 \\end{bmatrix} \\begin{bmatrix} -3 & -2 \\end{bmatrix}} = \\frac{16}{5}\n",
    "$"
   ]
  }
 ],
 "metadata": {
  "language_info": {
   "name": "python"
  }
 },
 "nbformat": 4,
 "nbformat_minor": 5
}
